nola/examples/rust_halt/num.v
@@ -7,24 +7,26 @@ Section num.
     !Jsem JUDG (iProp Σ)}.
 
   (** [ty_int]: Integer type *)
-  Definition pty_int : pty CON Σ Zₓ := λ n vl, ⌜vl = [ #n]⌝%cif.
+  Definition pty_int : pty CON Σ Zₓ := pair 1 (λ (n : Z) vl, ⌜vl = [ #n]⌝%cif).
   Definition ty_int : ty CON Σ Zₓ := ty_pty pty_int.
   (** [pty_int] satisfies [Pty] *)
-  #[export] Instance pty_int_pty : Pty pty_int 1.
+  #[export] Instance pty_int_pty : Pty pty_int.
   Proof. split=>/= *; [exact _|]. by iIntros "->". Qed.
 
   (** [ty_nat]: Natural number type *)
-  Definition pty_nat : pty CON Σ natₓ := λ n vl, ⌜vl = [ #n]⌝%cif.
+  Definition pty_nat : pty CON Σ natₓ :=
+    pair 1 (λ (n : nat) vl, ⌜vl = [ #n]⌝%cif).
   Definition ty_nat : ty CON Σ natₓ := ty_pty pty_nat.
   (** [pty_nat] satisfies [Pty] *)
-  #[export] Instance ty_nat_pty : Pty pty_nat 1.
+  #[export] Instance ty_nat_pty : Pty pty_nat.
   Proof. split=>/= *; [exact _|]. by iIntros "->". Qed.
 
   (** [ty_bool]: Boolean type *)
-  Definition pty_bool : pty CON Σ boolₓ := λ b vl, ⌜vl = [ #b]⌝%cif.
+  Definition pty_bool : pty CON Σ boolₓ :=
+    pair 1 (λ (b : bool) vl, ⌜vl = [ #b]⌝%cif).
   Definition ty_bool : ty CON Σ boolₓ := ty_pty pty_bool.
   (** [pty_bool] satisfies [Pty] *)
-  #[export] Instance ty_bool_pty : Pty pty_bool 1.
+  #[export] Instance ty_bool_pty : Pty pty_bool.
   Proof. split=>/= *; [exact _|]. by iIntros "->". Qed.
 
   (** Trivial resolution over numeric types *)
